# Chapter 1
## Intermission: Equivalence Exercises
We’ll give you a lambda expression. Keeping in mind both alpha equivalence and how multiple heads are nested, choose an answer that is equivalent to the listed lambda term

1. 𝜆𝑥𝑦.𝑥𝑧

  b) 𝜆𝑚𝑛.𝑚𝑧

2. 𝜆𝑥𝑦.𝑥𝑥𝑦

  c) 𝜆𝑎(𝜆𝑏.𝑎𝑎𝑏)

3. 𝜆𝑥𝑦𝑧.𝑧𝑥 

  b) 𝜆𝑡𝑜𝑠.𝑠`

## Chapter Exercises
### Combinators
Determine if each of the following are combinators or not.

Since "A combinator is a lambda term with no free variables":

1. 𝜆𝑥.𝑥𝑥𝑥

  This is a combinator: every variable is bound.

2. 𝜆𝑥𝑦.𝑧𝑥

  This isn't a combinator: z isn't bound (while the fact that y is defined but not used is inconsequential).

3. 𝜆𝑥𝑦𝑧.𝑥𝑦(𝑧𝑥)

  This is a combinator: every variable is bound.

4. 𝜆𝑥𝑦𝑧.𝑥𝑦(𝑧𝑥𝑦)

  This is a combinator: every variable is bound.

5. 𝜆𝑥𝑦.𝑥𝑦(𝑧𝑥𝑦)

  This isn't a combinator: z isn't bound.

### Normal form or diverge?
Determine if each of the following can be reduced to a normal form or if they diverge.

1. 𝜆𝑥.𝑥𝑥𝑥

  Can't be reduced more; it doesn't diverge, so it's in normal form.

2. (𝜆𝑧.𝑧𝑧)(𝜆𝑦.𝑦𝑦)

  Becomes `(𝜆[z := 𝜆𝑦.𝑦𝑦].𝑧𝑧) => (𝜆𝑦.𝑦𝑦)(𝜆𝑦.𝑦𝑦)`

  We're back to where we started. This doesn't converge to normal form, so it diverges.

3. (𝜆𝑥.𝑥𝑥𝑥)𝑧
  Becomes: `(𝜆[𝑥 := z].𝑥𝑥𝑥) => zzz`

  Can't be reduced more; it doesn't diverge, so it's in normal form.

### Beta reduce
Evaluate (that is, beta reduce) each of the following expressions to normal form. We strongly recommend writing out the steps on paper with a pencil or pen.

1. (𝜆𝑎𝑏𝑐.𝑐𝑏𝑎)𝑧𝑧(𝜆𝑤𝑣.𝑤)

```
(𝜆𝑎.𝜆𝑏.𝜆𝑐.𝑐𝑏𝑎)(𝑧)(𝑧)(𝜆𝑤.𝜆𝑣.𝑤)
(𝜆[𝑎 := z].𝜆𝑏.𝜆𝑐.𝑐𝑏𝑎)(𝑧)(𝜆𝑤.𝜆𝑣.𝑤)
(𝜆𝑏.𝜆𝑐.𝑐𝑏z)(𝑧)(𝜆𝑤.𝜆𝑣.𝑤)
(𝜆[𝑏 := z].𝜆𝑐.𝑐𝑏z)(𝜆𝑤.𝜆𝑣.𝑤)
(𝜆𝑐.𝑐zz)(𝜆𝑤.𝜆𝑣.𝑤)
(𝜆[𝑐 := (𝜆𝑤.𝜆𝑣.𝑤)].𝑐zz)
(𝜆𝑤.𝜆𝑣.𝑤)zz
(𝜆𝑤.𝜆𝑣.𝑤)(z)(z)
(𝜆[𝑤 := z].𝜆𝑣.𝑤)(z)
(𝜆𝑣.z)(z)
(𝜆[𝑣 := z].z)
z
```

2. (𝜆𝑥.𝜆𝑦.𝑥𝑦𝑦)(𝜆𝑎.𝑎)𝑏

```
(𝜆[x := (𝜆𝑎.𝑎)].𝜆𝑦.𝑥𝑦𝑦)𝑏
(𝜆𝑦.(𝜆𝑎.𝑎)𝑦𝑦)𝑏
(𝜆[𝑦 := 𝑏].(𝜆𝑎.𝑎)𝑦𝑦)
(𝜆𝑎.𝑎)bb
(𝜆𝑎.𝑎)(b)(b)
(𝜆[𝑎 := b].𝑎)(b)
(b)(b)
bb
```

3. (𝜆𝑦.𝑦)(𝜆𝑥.𝑥𝑥)(𝜆𝑧.𝑧𝑞)

```
(𝜆[𝑦 := (𝜆𝑥.𝑥𝑥)].𝑦)(𝜆𝑧.𝑧𝑞)
(𝜆𝑥.𝑥𝑥)(𝜆𝑧.𝑧𝑞)
(𝜆[𝑥 := (𝜆𝑧.𝑧𝑞)].𝑥𝑥)
(𝜆𝑧.𝑧𝑞)(𝜆𝑧.𝑧𝑞)
(𝜆[𝑧 := (𝜆𝑧.𝑧𝑞)].𝑧𝑞)
(𝜆𝑧.𝑧𝑞)𝑞
(𝜆[𝑧 := 𝑞].𝑧𝑞)
𝑞𝑞
```

4. (𝜆𝑧.𝑧)(𝜆𝑧.𝑧𝑧)(𝜆𝑧.𝑧𝑦) Hint: alpha equivalence.

```
(𝜆[𝑧 := (𝜆𝑧.𝑧𝑧)].𝑧)(𝜆𝑧.𝑧𝑦) -> We can jump this passage by noticing that the first function is the identity function: the output is the input
(𝜆𝑧.𝑧𝑧)(𝜆𝑧.𝑧𝑦)
(𝜆[𝑧 := (𝜆𝑧.𝑧𝑦)].𝑧𝑧)
(𝜆𝑧.𝑧𝑦)(𝜆𝑧.𝑧𝑦)
(𝜆[𝑧 := (𝜆𝑧.𝑧𝑦)].𝑧𝑦)
(𝜆𝑧.𝑧𝑦)𝑦
(𝜆[𝑧 := 𝑦].𝑧𝑦)
𝑦𝑦
```

5. (𝜆𝑥.𝜆𝑦.𝑥𝑦𝑦)(𝜆𝑦.𝑦)𝑦

```
(𝜆[𝑥 := (𝜆𝑦.𝑦)].𝜆𝑦.𝑥𝑦𝑦)𝑦
(𝜆𝑦.(𝜆𝑦.𝑦)𝑦𝑦)𝑦
(𝜆[𝑦 := y].(𝜆𝑦.𝑦)𝑦𝑦)
(𝜆𝑦.𝑦)𝑦𝑦
(𝜆𝑦.𝑦)(𝑦)(𝑦) -> identity function again
(𝑦)(𝑦)
𝑦𝑦
```

6. (𝜆𝑎.𝑎𝑎)(𝜆𝑏.𝑏𝑎)𝑐

```
(𝜆[𝑎 := (𝜆𝑏.𝑏𝑎)].𝑎𝑎)𝑐
(𝜆𝑏.𝑏𝑎)(𝜆𝑏.𝑏𝑎)𝑐
(𝜆[𝑏 := (𝜆𝑏.𝑏𝑎)].𝑏𝑎)𝑐
((𝜆𝑏.𝑏𝑎)(𝑎))𝑐
((𝜆[𝑏 := 𝑎].𝑏𝑎))𝑐
(𝑎𝑎)𝑐
𝑎𝑎𝑐
```

7. (𝜆𝑥𝑦𝑧.𝑥𝑧(𝑦𝑧))(𝜆𝑥.𝑧)(𝜆𝑥.𝑎)

```
(𝜆𝑥.𝜆𝑦.𝜆𝑧.𝑥𝑧(𝑦𝑧))(𝜆𝑥.𝑧)(𝜆𝑥.𝑎)
(𝜆𝑥.𝜆𝑦.𝜆𝑧.𝑥𝑧(𝑦𝑧))(𝜆𝑥.𝑧')(𝜆𝑥.𝑎)
(𝜆[𝑥 := (𝜆𝑥.𝑧')].𝜆𝑦.𝜆𝑧.𝑥𝑧(𝑦𝑧))(𝜆𝑥.𝑎)
(𝜆𝑦.𝜆𝑧.(𝜆𝑥.𝑧')𝑧(𝑦𝑧))(𝜆𝑥.𝑎)
(𝜆[𝑦 := (𝜆𝑥.𝑎)].𝜆𝑧.(𝜆𝑥.𝑧')𝑧(𝑦𝑧))
(𝜆𝑧.(𝜆𝑥.𝑧')𝑧((𝜆𝑥.𝑎)𝑧))
(𝜆𝑧.(𝜆[𝑥 := 𝑧].𝑧')((𝜆𝑥.𝑎)𝑧))
(𝜆𝑧.𝑧'((𝜆𝑥.𝑎)𝑧))
(𝜆𝑧.𝑧'((𝜆[𝑥 := 𝑧].𝑎)))
(𝜆𝑧.𝑧'((𝑎)))
𝜆𝑧.𝑧'𝑎
```